Isabelle2/AbstractMultiPaxosCorrectness.thy
@@ -5,9 +5,8 @@ imports AbstractMultiPaxos7 "../../IO-Automata/Simulations" "../../IO-Automata/I
   BallotArrayProperties
 begin
 
-locale amp_proof = IOA + quorums acceptors quorums + 
-    amp_ioa acceptors quorums learners for acceptors :: "'a set" 
-    and quorums and learners :: "'l set" +
+locale amp_proof = IOA + quorums quorums + amp_ioa quorums learners for 
+     quorums and learners :: "'l set" +
   fixes the_ioa :: "(('v,'a)amp_state, ('v,'a,'l)amp_action) ioa"
   defines "the_ioa \<equiv> amp_ioa"
 begin
@@ -22,16 +21,12 @@ declare amp_ioa_defs[inv_proofs_defs]
 declare the_ioa_def[inv_proofs_defs]
 
 declare propose_def[simp] join_ballot_def[simp] do_vote_def[simp]
-  learn_def[simp]
+  learn_def[simp] Let_def[simp] split_if[split] split_if_asm[split]
 
 lemma vote_one_inst_only:
   assumes "do_vote a i q v s s'" and "i \<noteq> j"
   shows "vote s j a = vote s' j a "
-using assms
-apply auto
-    apply (case_tac "ballot s a")
-apply auto
-done
+using assms by auto
 
 lemma vote_ballot_unch:
   assumes "do_vote a i q v s s'"
@@ -53,7 +48,7 @@ apply (try_solve_inv2 inv_proofs_defs:inv_proofs_defs invs:invs)
 done
 declare conservative_inductive[invs]
 
-subsection {* @{term safe}  is an inductive invariant*}
+subsection {* @{term safe}  is an inductive invariant *}
 
 abbreviation safe_at where "safe_at s i \<equiv> ballot_array.safe_at (ballot s) (vote s i) quorums"
 
@@ -63,79 +58,46 @@ lemma trans_imp_prefix_order:
 by (cases a) (auto simp add:is_prefix_def inv_proofs_defs split add:option.split_asm)
     
 lemma safe_mono:
-  -- {* @{term safe_at} is monotonic *}
+  -- {* @{term safe_at} is monotonic. TODO: needed? *}
   assumes "s \<midarrow>a\<midarrow>the_ioa\<longrightarrow> t" and "safe_at s i v b"
   shows "safe_at t i v b" using assms 
   by (drule_tac trans_imp_prefix_order)
    (metis (full_types) assms(1) ballot_array_prefix.safe_at_mono ballot_array_prefix_def trans_imp_prefix_order)
-  
-abbreviation safe where "safe s \<equiv> \<forall> i . ballot_array.safe (ballot s) (vote s i) quorums acceptors"
+
+abbreviation safe where "safe s \<equiv> \<forall> i . ballot_array.safe (ballot s) (vote s i) quorums"
 
 lemma safe_inv:
   "invariant the_ioa safe"
-apply(rule invariantI)
-    apply (force simp add:ballot_array.safe_def inv_proofs_defs)
-  apply instantiate_invs_2
-  apply (case_tac a)
-        (* propose *)
-        apply (force simp add:ballot_array.safe_def inv_proofs_defs ballot_array.safe_at_def ballot_array.choosable_def)
-      (* learn *)
-      apply (force simp add:ballot_array.safe_def inv_proofs_defs ballot_array.safe_at_def ballot_array.choosable_def)
-    (* vote *)
-    subgoal premises prems for s t act a q i v
-    proof (auto simp add:ballot_array.safe_def Let_def split add:option.split)
-      fix j b a\<^sub>2 v\<^sub>2
-      assume 1:"a\<^sub>2 \<in> acceptors" and 2:"vote t j a\<^sub>2 b = Some v\<^sub>2"
-      have l:"safe_at t j v\<^sub>2 b" if  "vote s j a\<^sub>2 b = vote t j a\<^sub>2 b"
-      proof -
-        have "safe_at s j v\<^sub>2 b" using that 1 2 prems(1) by (simp add:ballot_array.safe_def split add:option.split_asm)
-        thus ?thesis using prems(2) safe_mono by blast
-      qed
-      show "safe_at t j v\<^sub>2 b"
-      proof (cases "i = j \<and> a\<^sub>2 = a")
-        case False
-        have "vote s j a\<^sub>2 b = vote t j a\<^sub>2 b" using False prems(2,5) vote_one_inst_only
-          by (auto simp add:is_trans_def the_ioa_def amp_ioa_def amp_trans_def split add:option.split_asm)
-        with l show ?thesis by auto
-      next
-        case True
-        have 6:"do_vote a\<^sub>2 j q v s t" using prems(2,5) 1 True by (auto simp add:inv_proofs_defs)
-        with this obtain b\<^sub>2 where 3:"ballot s a\<^sub>2 = Some b\<^sub>2" and 4:"proved_safe_at s j q b\<^sub>2 v"
-        and 5:"t = s\<lparr>vote := (vote s)(j := (vote s j)(a\<^sub>2 := (vote s j a\<^sub>2)(b\<^sub>2 := Some v)))\<rparr>"
-        and 7:"\<And> a2 . a2 \<in> q \<Longrightarrow> ballot s a2 \<ge> Some b\<^sub>2" and 8:"q \<in> quorums"
-          by (auto split add:option.split_asm)
-        have ?thesis if "b \<noteq> b\<^sub>2"
-        proof -
-          have "vote s j a\<^sub>2 b = vote t j a\<^sub>2 b" using 5
-            by (smt amp_state.ext_inject amp_state.surjective amp_state.update_convs(3) fun_upd_apply that) 
-          with l show ?thesis by auto
-        qed
-        moreover have ?thesis if "b = b\<^sub>2"
-        proof -
-          have "v = v\<^sub>2" using that True
-            by (smt "2" "5" amp_state.ext_inject amp_state.surjective amp_state.update_convs(3) fun_upd_apply map_upd_Some_unfold)
-          hence 9:"vote t j a\<^sub>2 b = Some v\<^sub>2" using 5 that by force
-          hence "safe_at s j v\<^sub>2 b\<^sub>2" thm ballot_array_props.proved_safe_at_imp_safe_at
-            using ballot_array_props.proved_safe_at_imp_safe_at[of quorums acceptors  b\<^sub>2 "(vote s j)" "ballot s"  q v] 4 3 7 8 prems(1,3) that `v = v\<^sub>2`
-            apply auto 
-          with safe_mono prems(2) that True show ?thesis by blast
-        qed
-        ultimately show ?thesis by auto
-      qed
-    qed
-  (* join_ballot *)
-  subgoal premises prems for s t act a b
-  proof (auto simp add:ballot_array.safe_def split add:option.split)
-    fix i b\<^sub>2 a\<^sub>2 v
-    assume "vote t i a\<^sub>2 b\<^sub>2 = Some v" and "a\<^sub>2 \<in> acceptors"
-    note 1 = this
-    have 2:"vote t i a\<^sub>2 b\<^sub>2 = vote s i a\<^sub>2 b\<^sub>2" using prems(2,5) by (auto simp add:inv_proofs_defs)
-    hence 3:"safe_at s i v b\<^sub>2" using 1 prems(1)
-      by (metis ballot_array.safe_def option.simps(5)) 
-    with safe_mono prems(2,5)
-    show "safe_at t i v b\<^sub>2" apply (auto simp add:inv_proofs_defs)
-      by (metis amp_proof.safe_mono amp_proof_axioms amp_state.select_convs(3) amp_state.simps(2) amp_state.surjective amp_state.update_convs(2) prems(2) the_ioa_def) 
+apply (try_solve_inv2 inv_proofs_defs:inv_proofs_defs ballot_array.safe_def invs:invs)
+subgoal premises prems for s t act
+proof (auto simp add:ballot_array.safe_def split add:option.splits)
+  fix i b a v
+  assume "vote t i a b = Some v"
+  show "safe_at t i v b"
+  proof (cases "vote s i a b = Some v")
+    case True
+    hence "safe_at s i v b" using prems(1) by (metis ballot_array.safe_def option.simps(5))
+    thus "safe_at t i v b" using prems(2) safe_mono by simp
+  next
+    case False
+    with prems(2) \<open>vote t i a b = Some v\<close> obtain q where "do_vote a i q v s t" and "ballot s a = b"
+      apply(simp add:is_trans_def the_ioa_def amp_ioa_def amp_trans_def del:do_vote_def)
+      apply(elim amp_trans_rel.elims)
+      apply simp
+      apply simp
+      defer
+      apply simp
+      apply (simp (no_asm_use))
+      apply (smt amp_ioa.do_vote_def amp_state.iffs amp_state.surjective amp_state.update_convs(3) fun_upd_apply option.sel)
+      done
+    hence "proved_safe_at s i q (ballot s a) v" and "q \<in> quorums" and "\<forall> a2 \<in> q . ballot s a \<le> ballot s a2" 
+      by (simp_all add:ballot_array.proved_safe_at_def split add:nat.splits)
+    hence "safe_at s i v b" using quorums_axioms prems(1) prems(3) `ballot s a = b`
+      ballot_array_props.proved_safe_at_imp_safe_at[of quorums "ballot s a" "vote s i" "ballot s" q v]
+      by (auto simp add:ballot_array.safe_def ballot_array_props_def split add:option.splits)
+    thus "safe_at t i v b" using prems(2) safe_mono by simp
   qed
+qed
 done
 declare safe_inv[invs]
 
@@ -149,7 +111,7 @@ apply(rule invariantI)
     apply(auto simp add: inv_proofs_defs agreement_def ballot_array.chosen_def ballot_array.chosen_at_def)[1]
     apply (metis empty_iff quorum_inter_witness)
   apply instantiate_invs_2
-  apply (meson agreement_def ballot_array_props.intro ballot_array_props.safe_is_safe quorums_axioms)
+  apply (meson agreement_def ballot_array_props.intro ballot_array_props.safe_imp_agreement quorums_axioms)
 done
 
 end
